Fix all files

examples/delayed_echo/EchoAll.v
@@ -17,6 +17,31 @@ Generalizable Variables E R A B C X Y Σ.
 Set Implicit Arguments.
 
 
+
+
+Section AUX________REMOVEME_____REDUNDANT.
+
+  Context `{Σ: GRA.t}.
+
+  Definition refines_closed (md_tgt md_src: ModL.t): Prop :=
+    Beh.of_program (ModL.compile md_tgt) <1= Beh.of_program (ModL.compile md_src)
+  .
+
+  Lemma refines_close: SimModSem.refines <2= refines_closed.
+  Proof. ii. specialize (PR nil). ss. unfold Mod.add_list in *. ss. rewrite ! ModL.add_empty_l in PR. eauto. Qed.
+
+  Definition add_list (ms: list ModL.t): ModL.t := fold_right ModL.add ModL.empty ms.
+
+  Global Program Instance refines_closed_PreOrder: PreOrder refines_closed.
+  Next Obligation. ii; ss. Qed.
+  Next Obligation. ii; ss. r in H. r in H0. eauto. Qed.
+
+End AUX________REMOVEME_____REDUNDANT.
+
+
+
+
+
 Section ECHO.
 
   Definition Σ: GRA.t := GRA.of_list [Mem1.memRA; Echo1.echoRA].
@@ -35,7 +60,7 @@ Section ECHO.
   Local Existing Instance echoRA_inG.
 
   Definition echo_spec: ModL.t :=
-    ModL.add_list [
+    add_list [
         md_src Mem MemSbtb ; (* Mem *)
         md_src Main MainSbtb ; (* Main *)
         md_src Stack StackSbtb ; (* Stack *)
