examples/mem/Main0.v
@@ -49,7 +49,8 @@ Section PROOF.
 
   Definition Main: Mod.t := {|
     Mod.get_modsem := fun _ => MainSem;
-    Mod.sk := Sk.unit;
+    (* Mod.sk := Sk.unit; *)
+    Mod.sk := [("main", Sk.Gfun)];
   |}
   .
 End PROOF.
