examples/mem/MemMain.v
@@ -15,7 +15,7 @@ Set Implicit Arguments.
 
 
 
-Require Import Mem0 Mem1 Main0 Main1.
+Require Import Mem0 Mem1 Mem01proof Main0 Main1.
 
 
 
@@ -49,7 +49,7 @@ Section MEM2.
   Context `{@GRA.inG memRA Σ}.
 
   Definition MemSem: ModSem.t := {|
-    ModSem.fnsems := List.map (fun '(fn, fsb) => (fn, fun_to_tgt (MainStb++MemStb) fn fsb)) MemSbtb;
+    ModSem.fnsems := List.map (fun '(fn, fsb) => (fn, fun_to_tgt (MemStb ++ MainStb) fn fsb)) MemSbtb;
     ModSem.mn := "Mem";
     ModSem.initial_mr := (GRA.embed (Auth.black (M:=Mem1._memRA) ε));
     ModSem.initial_st := tt↑;
@@ -58,7 +58,7 @@ Section MEM2.
 
   Definition Mem: Mod.t := {|
     Mod.get_modsem := fun _ => MemSem;
-    Mod.sk := List.map (fun '(n, _) => (n, Sk.Gfun)) MemStb;
+    Mod.sk := Sk.unit;
   |}
   .
 
@@ -77,7 +77,7 @@ Section WEAKENING.
   Let weaken: forall (fn fn_tgt : string) (fsp_tgt : fspec),
       find (fun '(_fn, _) => dec fn _fn) MemStb = Some (fn_tgt, fsp_tgt) ->
       exists (fn_src : string) (fsp_src : fspec),
-        (<< _ : find (fun '(_fn, _) => dec fn _fn) (MainStb ++ MemStb) = Some (fn_src, fsp_src) >>) /\ << _ : fspec_weaker fsp_tgt fsp_src >>
+        (<< _ : find (fun '(_fn, _) => dec fn _fn) (MemStb ++ MainStb) = Some (fn_src, fsp_src) >>) /\ << _ : fspec_weaker fsp_tgt fsp_src >>
   .
   Proof.
     ii. stb_tac. des_ifs.
@@ -133,6 +133,37 @@ End WEAKENING.
 
 
 
+Section AUX.
+
+  Theorem GRA_wf_embed
+          A
+          `{@GRA.inG A Σ}
+          (a: A)
+          (WF: URA.wf a)
+    :
+      URA.wf (GRA.embed a)
+  .
+  Proof.
+    ss. ii. unfold GRA.embed.
+    Local Transparent GRA.to_URA. ur. i. des_ifs; cycle 1.
+    { apply URA.wf_unit. }
+    ss. unfold PCM.GRA.cast_ra, eq_rect, eq_sym. destruct GRA.inG_prf. ss.
+    Local Opaque GRA.to_URA.
+  Qed.
+
+  Theorem Auth_wf_black
+          `{M: URA.t}
+          a
+          (WF: URA.wf a)
+    :
+      <<WF: URA.wf (Auth.black a)>>
+  .
+  Proof. ur. split; ss. r. esplits. rewrite URA.unit_idl. refl. Qed.
+
+End AUX.
+
+
+
 
 Section PROOF.
 
@@ -178,174 +209,82 @@ Section PROOF.
   |}
   .
 
-  Theorem correct: refines_closed MemMain1 MemMain2.
+  Let sbtb_stb: (MemStb ++ MainStb) = List.map (fun '(gn, fsb) => (gn, fsb.(fsb_fspec))) (MemSbtb ++ MainSbtb).
+  Proof. rewrite map_app. ss. unfold MainStb, MemStb. unseal "stb". refl. Qed.
+
+  Theorem correct12: refines_closed MemMain1 MemMain2.
   Proof.
     r.
     set (global_sbtb:=MemSbtb++MainSbtb).
     Local Opaque MemSbtb.
     Local Opaque MainSbtb.
     eapply adequacy_type with (sbtb:=global_sbtb).
-    { unfold compose. cbn. f_equal.
-    eapply adequacy_type.
-  Qed.
-
-  Theorem embed_wf
-          A
-          `{@GRA.inG A Σ}
-          (a: A)
-          (WF: URA.wf a)
-    :
-      URA.wf (GRA.embed a)
-  .
-  Proof.
-    ss. ii. unfold GRA.embed.
-    Local Transparent GRA.to_URA. ur. i. des_ifs; cycle 1.
-    { apply URA.wf_unit. }
-    ss. unfold PCM.GRA.cast_ra, eq_rect, eq_sym. destruct GRA.inG_prf. ss.
-    Local Opaque GRA.to_URA.
-  Qed.
-
-  (* Definition incl (sbtb0 sbtb1: list (string * fspec)): Prop := List.incl  *)
-  (* Lemma handle_hCallE_tgt_ext *)
-  (*       sbtb0 sbtb1 mn cur *)
-  (*   : *)
-  (*     (handle_hCallE_tgt sbtb0 mn cur) = (handle_hCallE_tgt sbtb1 mn cur) *)
-  (* . *)
-  (* Proof. *)
-  (*   unfold handle_hCallE_tgt. repeat (apply func_ext_dep; i). des_ifs. *)
-  (*   - *)
-  (* Qed. *)
-
-  (* Let body_to_tgt_aux: forall E R1 R2 RR *)
-  (*     AR sbtb0 sbtb1 mn cur *)
-  (*     (bd: itree (hCallE +' pE +' eventE) AR) *)
-  (*     i_src i_tgt *)
-  (*     (SRC: i_src ~= (interp_hCallE_tgt sbtb0 mn cur bd)) *)
-  (*     (TGT: i_tgt ~= (interp_hCallE_tgt sbtb1 mn cur bd)) *)
-  (*   , *)
-  (*     @eq_itree E R1 R2 RR i_src i_tgt *)
-  (* (* ≅  *) *)
-  (* . *)
-  (* Proof. *)
-  (*   ginit. *)
-  (*   ecofix CIH. *)
-  (* Qed. *)
-  (* Unset Universe Checking. *)
-
-
-
-  (*********** TODO: finish the theory and move to proper place ***********)
-  Definition contains R (stb: list (string * fspec)) (body: itree (hCallE +' pE +' eventE) R): Prop :=
-    admit "fspecbody's body calls only the functions that are inside stb"
-  .
-
-  Definition extends (stb0 stb1: list (string * fspec)): Prop :=
-    (* admit "stb1 has more entries" *)
-    List.incl stb0 stb1
-  .
-
-  Lemma interp_hCallE_tgt_ext
-        AR
-        stb0 stb1 mn cur (body: itree (hCallE +' pE +' eventE) AR)
-        (A: contains stb0 body)
-        (B: extends stb0 stb1)
-    :
-      interp_hCallE_tgt stb0 mn cur body = interp_hCallE_tgt stb1 mn cur body
-  .
-  Proof.
-    f. ginit. revert_until Σ. gcofix CIH. i.
-    unfold interp_hCallE_tgt.
-    ides body;  rewrite ! unfold_interp; ired; ss.
-    - gstep. econs; et.
-    - gstep. econs; et. gbase. eapply CIH; ss.
-    - guclo eqit_clo_bind. econs.
-      + instantiate (1:=eq). destruct e.
-        { (**** main part ****)
-          ired. unfold handle_hCallE_tgt.
-          unfold unwrapN. des_ifs.
-          - assert(T: p = p0) by admit "ez - uniqueness". subst. refl.
-          - exfalso. admit "ez - extends".
-          - exfalso. admit "ez - contains".
-          - exfalso. admit "ez - contains".
-        }
-        destruct s; ss.
-        { destruct p; ss; ired; refl. }
-        { destruct e; ss; ired; refl. }
-      + ii. clarify. gstep. econs; eauto. gbase. eapply CIH; et.
-  Unshelve.
-    all: try (by econs).
-  Qed.
-
-  Lemma body_to_tgt_ext
-        AA AR
-        stb0 stb1 mn cur (body: (AA -> itree (hCallE +' pE +' eventE) AR)) varg
-        (A: contains stb0 (body varg))
-        (B: extends stb0 stb1)
-    :
-      body_to_tgt stb0 mn cur body varg = body_to_tgt stb1 mn cur body varg
-  .
-  Proof. eapply interp_hCallE_tgt_ext; et. Qed.
-
-  Lemma fun_to_tgt_ext
-        stb0 stb1 fn sb
-        (A: forall varg, contains stb0 (sb.(fsb_body) varg))
-        (B: extends stb0 stb1)
-    :
-      fun_to_tgt stb0 fn sb = fun_to_tgt stb1 fn sb
-  .
-  Proof.
-    unfold fun_to_tgt. unfold HoareFun. apply func_ext. i. grind.
-    erewrite body_to_tgt_ext; et. grind.
-    erewrite interp_hCallE_tgt_ext; et. eapply A; et.
-  Unshelve.
-    all: ss.
-  Qed.
-
-  (* Lemma map_ext *)
-  (*       A B *)
-  (*       l (f g : A -> B) *)
-  (*       (EXT: forall a, In a l -> f a = g a) *)
-  (*   : *)
-  (*     List.map f l = List.map g l *)
-  (* . *)
-  (* Proof. *)
-  (*   clear Σ H. *)
-  (*   ginduction l; ii; ss. f_equal. *)
-  (*   - eapply EXT; et. *)
-  (*   - eapply IHl; et. *)
-  (* Qed. *)
-
-  Theorem correct: Beh.of_program (Mod.compile MemMain1) <1= Beh.of_program (Mod.compile MemMain2).
-  Proof.
-    ii.
-    set (global_sbtb:=MemSbtb++MainSbtb).
-    (* clearbody global_stb. *)
-    Local Opaque MemSbtb.
-    Local Opaque MainSbtb.
-    eapply adequacy_type with (sbtb:=global_sbtb) in PR.
-    { ss. }
-    { cbn. unfold global_sbtb. rewrite List.map_app.
-      Set Printing Coercions.
-      seal fun_to_tgt. (*** without this, other tactics (des_ifs; refl; ss; f_equal; etc) will take infinite time. Opaque does help here at all. ***)
-      f_equal; cycle 1.
-      { autounfold with stb; autorewrite with stb; refl. }
-      apply map_ext. (*** better than just "f_equal" ***)
-      i. des_ifs. r; f_equal. unseal fun_to_tgt. eapply fun_to_tgt_ext.
-      - ii. ss.
-        Local Transparent MemSbtb. cbn in IN. Local Opaque MemSbtb. des; ss; clarify; ss.
-        + admit "ez".
-        + admit "ez".
-        + admit "ez".
-        + admit "ez".
-        + admit "ez".
-      - admit "ez".
+    { seal fun_to_tgt. unfold compose. cbn. unfold global_sbtb. rewrite map_app. unfold ModSem.map_snd.
+      f_equal.
+      - rewrite List.map_map. eapply map_ext. ii. des_ifs. r. f_equal. apply func_ext. i. f_equal.
+        + Local Transparent MemSbtb. cbn in IN. Local Opaque MemSbtb.
+          des; ss; clarify; ss.
+        + unseal fun_to_tgt. f_equal. ss.
+      - rewrite List.map_map. eapply map_ext. ii. des_ifs. r. f_equal. apply func_ext. i. f_equal.
+        + Local Transparent MainSbtb. cbn in IN. Local Opaque MainSbtb.
+          des; ss; clarify; ss.
+        + unseal fun_to_tgt. f_equal. ss.
     }
-    { Local Transparent MemSbtb. cbn. Local Opaque MemSbtb. des_ifs; ss. }
-    ss. unfold compose. ss. rewrite ! URA.unit_id. rewrite ! URA.unit_idl.
-    eapply embed_wf; et.
-    assert(@URA.wf (Mem1._memRA) (fun b ofs => if (b =? 0)%nat && (ofs =? 0)%Z then Excl.just Vundef else Excl.unit)).
-    { repeat ur. i; des_ifs. }
-    admit "EZ -- add black wf lemma".
+    { ss. }
+    { ss. }
+    { instantiate (1:=ε). des_ifs. ss. unfold compose, ModSemL.initial_r_state in *. des_ifs.
+      rewrite ! URA.unit_idl. ss. rewrite ! URA.unit_id. eapply GRA_wf_embed. eapply Auth_wf_black.
+      repeat ur. i; ss.
+    }
+  Qed.
+
+  Theorem correct: refines_closed MemMain0 MemMain2.
+  Proof.
+    etrans; cycle 1.
+    { eapply correct12. }
+    etrans; cycle 1.
+    { instantiate (1:=ModL.add Mem1.Mem Main1.Main).
+      eapply refines_close.
+      hexploit (SimModSem.refines_proper_r [Mem2.Mem] [Mem1.Mem] [Main1.Main]).
+      { cbn. rewrite ! ModL.add_empty_r. eapply SimModSem.adequacy_local.
+        econs.
+        - i. cbn. eapply SimModSem.adequacy_lift. eapply Mem12correct.
+        - ss.
+        - cbn. ii. rr. econs; ss.
+          { repeat (econs; ii; ss; des; ss). }
+          { repeat (econs; ii; ss; des; ss). }
+      }
+      intro T; des. cbn in T. rewrite ! ModL.add_empty_r in T. ss.
+    }
+    etrans; cycle 1.
+    { instantiate (1:=ModL.add Mem0.Mem Main1.Main).
+      eapply refines_close.
+      hexploit (SimModSem.refines_proper_r [Mem1.Mem] [Mem0.Mem] [Main1.Main]).
+      { cbn. rewrite ! ModL.add_empty_r. eapply SimModSem.adequacy_local.
+        econs.
+        - i. cbn. eapply SimModSem.adequacy_lift. eapply Mem01proof.correct.
+        - ss.
+        - cbn. ii. rr. econs; ss.
+          { repeat (econs; ii; ss; des; ss). }
+          { repeat (econs; ii; ss; des; ss). }
+      }
+      intro T; des. cbn in T. rewrite ! ModL.add_empty_r in T. ss.
+    }
+    etrans; cycle 1.
+    { instantiate (1:=ModL.add Mem0.Mem Main0.Main).
+      eapply refines_close.
+      hexploit (SimModSem.refines_proper_l [Main1.Main] [Main0.Main] [Mem0.Mem]).
+      { cbn. rewrite ! ModL.add_empty_r. eapply SimModSem.adequacy_local.
+        econs.
+        - i. cbn. eapply SimModSem.adequacy_lift. admit "should be ez".
+        - ss.
+        - cbn. ii. rr. econs; ss.
+          { repeat (econs; ii; ss; des; ss). }
+          { repeat (econs; ii; ss; des; ss). }
+      }
+      intro T; des. cbn in T. rewrite ! ModL.add_empty_r in T. ss.
+    }
+    refl.
   Qed.
 
 End PROOF.
